io/IIO.fst
@@ -47,31 +47,6 @@ let dm_iio_subcomp a wp1 wp2 f = dm_subcomp iio_cmds iio_sig event iio_wps a wp1
 
 (** ** Types **)
 
-(** **** Tree **)
-type tree (a: Type) =
-  | Leaf : tree a
-  | EmptyNode: left: tree a -> right: tree a -> tree a
-  | Node: data: a -> left: tree a -> right: tree a -> tree a
-
-let root (t:(tree 'a){Node? t}) = Node?.data t
-let eleft (t:(tree 'a){EmptyNode? t}) = EmptyNode?.left t
-let eright (t:(tree 'a){EmptyNode? t}) = EmptyNode?.right t
-let left (t:(tree 'a){Node? t}) = Node?.left t
-let right (t:(tree 'a){Node? t}) = Node?.right t
-
-let rec equal_trees (t1:tree 'a) (t2:tree 'a) =
-  match t1, t2 with
-  | Leaf, Leaf -> True
-  | EmptyNode lhs1 rhs1, EmptyNode lhs2 rhs2 -> equal_trees lhs1 lhs2 /\ equal_trees rhs1 rhs2
-  | Node x lhs1 rhs1, Node y lhs2 rhs2 -> x == y /\ equal_trees lhs1 lhs2 /\ equal_trees rhs1 rhs2
-  | _, _ -> False
-
-let rec map_tree (t:tree 'a) (f:'a -> 'b) : tree 'b =
-  match t with
-  | Leaf -> Leaf 
-  | EmptyNode lhs rhs -> EmptyNode (map_tree lhs f) (map_tree rhs f)
-  | Node x lhs rhs -> Node (f x) (map_tree lhs f) (map_tree rhs f)
-
 (** **** Flag **)
 noeq
 type tflag = | NoActions | GetTraceActions | IOActions | AllActions
